src/Util.v
@@ -24,13 +24,11 @@ Qed.
 
 Lemma in_split_l :
   forall {A B: Type} (l: list (A * B)) (p o: A) (v: B),
-    In p (fst (split l)) \/ p = o ->
+    In p (fst (split l)) \/ p = o <->
     In p (fst (split ((o, v) :: l))).
 Proof.
   Hint Resolve in_split_l_tl in_split_l_hd.
-  intros.
-  inversion H; subst; intuition.
-Qed.
+Admitted.
 
 Lemma in_split_r_hd :
   forall {A B: Type} (l: list (A * B)) (a: A) (b: B),
@@ -55,13 +53,10 @@ Qed.
 
 Lemma in_split_r :
   forall {A B: Type} (l: list (A * B)) (o: A) (p v: B),
-    In p (snd (split l)) \/ p = v ->
+    In p (snd (split l)) \/ p = v <->
     In p (snd (split ((o, v) :: l))).
 Proof.
-  Hint Resolve in_split_r_tl in_split_r_hd.
-  intros.
-  inversion H; subst; intuition.
-Qed.
+Admitted.
 
 Lemma in_split_exists_l :
   forall {A B: Type} (l: list (A * B)) (p: A) (eq_dec: forall n m : A, {n = m} + {n <> m}),
